extraction/src/ErgoParser.mly
@@ -30,7 +30,10 @@ let relative_ref_of_qname_base qn =
   let (prefix,localname) = qname_of_qname_base qn in
   (prefix,localname)
 
-let mk_position (start_pos: Lexing.position) (end_pos: Lexing.position) : location = mk_position_of_loc_pair start_pos end_pos
+let mk_provenance
+    (start_pos: Lexing.position)
+    (end_pos: Lexing.position) : provenance =
+    mk_provenance_of_loc_pair start_pos end_pos
 %}
 
 %token <int> INT
@@ -99,7 +102,7 @@ main_decl:
 
 emodule:
 | NAMESPACE qn = qname_prefix ims = imports ss = decls
-    { { module_annot = mk_position $startpos $endpos;
+    { { module_annot = mk_provenance $startpos $endpos;
         module_namespace = Util.char_list_of_string qn;
         module_imports = ims;
         module_declarations = ss; } }
@@ -119,48 +122,48 @@ decls:
 decl:
 | DEFINE CONCEPT cn = ident dt = ergo_type_class_decl
     { let (oe,ctype) = dt in
-      ErgoCompiler.dtype (mk_position $startpos $endpos)
-        (ErgoCompiler.mk_ergo_type_declaration (mk_position $startpos $endpos) cn (ErgoTypeConcept (oe,ctype))) }
+      ErgoCompiler.dtype (mk_provenance $startpos $endpos)
+        (ErgoCompiler.mk_ergo_type_declaration (mk_provenance $startpos $endpos) cn (ErgoTypeConcept (oe,ctype))) }
 | DEFINE TRANSACTION cn = ident dt = ergo_type_class_decl
     { let (oe,ctype) = dt in
-      ErgoCompiler.dtype (mk_position $startpos $endpos)
-        (ErgoCompiler.mk_ergo_type_declaration (mk_position $startpos $endpos) cn (ErgoTypeTransaction (oe,ctype))) }
+      ErgoCompiler.dtype (mk_provenance $startpos $endpos)
+        (ErgoCompiler.mk_ergo_type_declaration (mk_provenance $startpos $endpos) cn (ErgoTypeTransaction (oe,ctype))) }
 | DEFINE ENUM cn = ident et = ergo_type_enum_decl
-    { ErgoCompiler.dtype (mk_position $startpos $endpos)
-        (ErgoCompiler.mk_ergo_type_declaration (mk_position $startpos $endpos) cn (ErgoTypeEnum et)) }
+    { ErgoCompiler.dtype (mk_provenance $startpos $endpos)
+        (ErgoCompiler.mk_ergo_type_declaration (mk_provenance $startpos $endpos) cn (ErgoTypeEnum et)) }
 | DEFINE CONSTANT v = ident EQUAL e = expr
-    { ErgoCompiler.dconstant (mk_position $startpos $endpos) v e }
+    { ErgoCompiler.dconstant (mk_provenance $startpos $endpos) v e }
 | DEFINE FUNCTION cn = ident LPAREN ps = params RPAREN COLON out = paramtype mt = maythrow LCURLY fs = fstmt RCURLY
-    { ErgoCompiler.dfunc (mk_position $startpos $endpos)
-        { function_annot = mk_position $startpos $endpos;
+    { ErgoCompiler.dfunc (mk_provenance $startpos $endpos)
+        { function_annot = mk_provenance $startpos $endpos;
           function_name = cn;
           function_sig =
-          { type_signature_annot = (mk_position $startpos $endpos);
+          { type_signature_annot = (mk_provenance $startpos $endpos);
             type_signature_params = ps;
             type_signature_output = out;
             type_signature_throws = fst mt;
             type_signature_emits = snd mt };
           function_body = Some fs; } }
 | DEFINE FUNCTION cn = ident LPAREN ps = params RPAREN COLON out = paramtype mt = maythrow
-    { ErgoCompiler.dfunc (mk_position $startpos $endpos)
-        { function_annot = mk_position $startpos $endpos;
+    { ErgoCompiler.dfunc (mk_provenance $startpos $endpos)
+        { function_annot = mk_provenance $startpos $endpos;
           function_name = cn;
           function_sig =
-          { type_signature_annot = (mk_position $startpos $endpos);
+          { type_signature_annot = (mk_provenance $startpos $endpos);
             type_signature_params = ps;
             type_signature_output = out;
             type_signature_throws = fst mt;
             type_signature_emits = snd mt };
           function_body = None; } }
 | CONTRACT cn = ident OVER tn = paramtype ms = mayhavestate LCURLY ds = clauses RCURLY
-    { ErgoCompiler.dcontract (mk_position $startpos $endpos)
-        { contract_annot = mk_position $startpos $endpos;
+    { ErgoCompiler.dcontract (mk_provenance $startpos $endpos)
+        { contract_annot = mk_provenance $startpos $endpos;
           contract_name = cn;
           contract_template = tn;
           contract_state = ms;
           contract_clauses = ds; } }
 | s = stmt SEMI
-    { ErgoCompiler.dstmt (mk_position $startpos $endpos) s }
+    { ErgoCompiler.dstmt (mk_provenance $startpos $endpos) s }
 
 ergo_type_class_decl:
 | LCURLY rt = rectype RCURLY
@@ -180,10 +183,10 @@ clauses:
 
 clause:
 | CLAUSE cn = ident LPAREN ps = params RPAREN COLON out = paramtype mt = maythrow LCURLY s = stmt RCURLY
-    { { clause_annot = mk_position $startpos $endpos;
+    { { clause_annot = mk_provenance $startpos $endpos;
         clause_name = cn;
         clause_sig =
-        { type_signature_annot = (mk_position $startpos $endpos);
+        { type_signature_annot = (mk_provenance $startpos $endpos);
           type_signature_params = ps;
           type_signature_output = out;
           type_signature_throws = fst mt;
@@ -216,30 +219,30 @@ params:
 
 param:
 | pn = IDENT
-    { (Util.char_list_of_string pn, ErgoCompiler.ergo_type_any (mk_position $startpos $endpos)) }
+    { (Util.char_list_of_string pn, ErgoCompiler.ergo_type_any (mk_provenance $startpos $endpos)) }
 | pn = IDENT COLON pt = paramtype
     { (Util.char_list_of_string pn, pt) }
 
 paramtype:
 | qn = qname_base
     { begin match qn with
-      | (None, "Boolean") -> ErgoCompiler.ergo_type_boolean (mk_position $startpos $endpos)
-      | (None, "String") -> ErgoCompiler.ergo_type_string (mk_position $startpos $endpos)
-      | (None, "Double") -> ErgoCompiler.ergo_type_double (mk_position $startpos $endpos)
-      | (None, "Long") -> ErgoCompiler.ergo_type_long (mk_position $startpos $endpos)
-      | (None, "Integer") -> ErgoCompiler.ergo_type_integer (mk_position $startpos $endpos)
-      | (None, "DateTime") -> ErgoCompiler.ergo_type_dateTime (mk_position $startpos $endpos)
-      | (None, "Empty") -> ErgoCompiler.ergo_type_none (mk_position $startpos $endpos)
-      | (None, "Any") -> ErgoCompiler.ergo_type_any (mk_position $startpos $endpos)
+      | (None, "Boolean") -> ErgoCompiler.ergo_type_boolean (mk_provenance $startpos $endpos)
+      | (None, "String") -> ErgoCompiler.ergo_type_string (mk_provenance $startpos $endpos)
+      | (None, "Double") -> ErgoCompiler.ergo_type_double (mk_provenance $startpos $endpos)
+      | (None, "Long") -> ErgoCompiler.ergo_type_long (mk_provenance $startpos $endpos)
+      | (None, "Integer") -> ErgoCompiler.ergo_type_integer (mk_provenance $startpos $endpos)
+      | (None, "DateTime") -> ErgoCompiler.ergo_type_dateTime (mk_provenance $startpos $endpos)
+      | (None, "Empty") -> ErgoCompiler.ergo_type_none (mk_provenance $startpos $endpos)
+      | (None, "Any") -> ErgoCompiler.ergo_type_any (mk_provenance $startpos $endpos)
       | _ ->
-          ErgoCompiler.ergo_type_class_ref (mk_position $startpos $endpos) (relative_ref_of_qname_base qn)
+          ErgoCompiler.ergo_type_class_ref (mk_provenance $startpos $endpos) (relative_ref_of_qname_base qn)
       end }
 | LCURLY rt = rectype RCURLY
-    { ErgoCompiler.ergo_type_record (mk_position $startpos $endpos) rt }
+    { ErgoCompiler.ergo_type_record (mk_provenance $startpos $endpos) rt }
 | pt = paramtype LBRACKET RBRACKET
-    { ErgoCompiler.ergo_type_array (mk_position $startpos $endpos) pt }
+    { ErgoCompiler.ergo_type_array (mk_provenance $startpos $endpos) pt }
 | pt = paramtype QUESTION
-    { ErgoCompiler.ergo_type_option (mk_position $startpos $endpos) pt }
+    { ErgoCompiler.ergo_type_option (mk_provenance $startpos $endpos) pt }
 
 rectype:
 | 
@@ -256,45 +259,45 @@ attributetype:
 stmt:
 (* Statments *)
 | RETURN
-    { ErgoCompiler.sreturnempty (mk_position $startpos $endpos) }
+    { ErgoCompiler.sreturnempty (mk_provenance $startpos $endpos) }
 | RETURN e1 = expr
-    { ErgoCompiler.sreturn (mk_position $startpos $endpos) e1 }
+    { ErgoCompiler.sreturn (mk_provenance $startpos $endpos) e1 }
 | THROW e1 = expr
-    { ErgoCompiler.sthrow (mk_position $startpos $endpos) e1 }
+    { ErgoCompiler.sthrow (mk_provenance $startpos $endpos) e1 }
 (* Call *)
 | fn = IDENT LPAREN el = exprlist RPAREN
-    { ErgoCompiler.scallclause (mk_position $startpos $endpos) (Util.char_list_of_string fn) el }
+    { ErgoCompiler.scallclause (mk_provenance $startpos $endpos) (Util.char_list_of_string fn) el }
 | LET v = ident EQUAL e1 = expr SEMI s2 = stmt
-    { ErgoCompiler.slet (mk_position $startpos $endpos) v e1 s2 }
+    { ErgoCompiler.slet (mk_provenance $startpos $endpos) v e1 s2 }
 | LET v = ident COLON t = paramtype EQUAL e1 = expr SEMI s2 = stmt
-    { ErgoCompiler.slet_typed (mk_position $startpos $endpos) v t e1 s2 }
+    { ErgoCompiler.slet_typed (mk_provenance $startpos $endpos) v t e1 s2 }
 | IF e1 = expr THEN s2 = stmt ELSE s3 = stmt
-    { ErgoCompiler.sif (mk_position $startpos $endpos) e1 s2 s3 }
+    { ErgoCompiler.sif (mk_provenance $startpos $endpos) e1 s2 s3 }
 | ENFORCE e1 = expr ELSE s2 = stmt SEMI s3 = stmt
-    { ErgoCompiler.senforce (mk_position $startpos $endpos) e1 (Some s2) s3 }
+    { ErgoCompiler.senforce (mk_provenance $startpos $endpos) e1 (Some s2) s3 }
 | ENFORCE e1 = expr SEMI s3 = stmt
-    { ErgoCompiler.senforce (mk_position $startpos $endpos) e1 None s3 }
+    { ErgoCompiler.senforce (mk_provenance $startpos $endpos) e1 None s3 }
 | SET STATE e1 = expr SEMI s2 = stmt
-    { ErgoCompiler.ssetstate (mk_position $startpos $endpos) e1 s2 }
+    { ErgoCompiler.ssetstate (mk_provenance $startpos $endpos) e1 s2 }
 | EMIT e1 = expr SEMI s2 = stmt
-    { ErgoCompiler.semit (mk_position $startpos $endpos) e1 s2 }
+    { ErgoCompiler.semit (mk_provenance $startpos $endpos) e1 s2 }
 | MATCH e0 = expr csd = cases_stmt
-    { ErgoCompiler.smatch (mk_position $startpos $endpos) e0 (fst csd) (snd csd) }
+    { ErgoCompiler.smatch (mk_provenance $startpos $endpos) e0 (fst csd) (snd csd) }
 
 fstmt:
 (* Statments *)
 | RETURN
-    { ErgoCompiler.sfunreturnempty (mk_position $startpos $endpos) }
+    { ErgoCompiler.sfunreturnempty (mk_provenance $startpos $endpos) }
 | RETURN e1 = expr
-    { ErgoCompiler.sfunreturn (mk_position $startpos $endpos) e1 }
+    { ErgoCompiler.sfunreturn (mk_provenance $startpos $endpos) e1 }
 | THROW e1 = expr
     { raise (LexError ("Cannot throw inside a function, you have to be in a Clause")) }
 | LET v = ident EQUAL e1 = expr SEMI s2 = fstmt
-    { ErgoCompiler.slet (mk_position $startpos $endpos) v e1 s2 }
+    { ErgoCompiler.slet (mk_provenance $startpos $endpos) v e1 s2 }
 | LET v = ident COLON t = paramtype EQUAL e1 = expr SEMI s2 = fstmt
-    { ErgoCompiler.slet_typed (mk_position $startpos $endpos) v t e1 s2 }
+    { ErgoCompiler.slet_typed (mk_provenance $startpos $endpos) v t e1 s2 }
 | IF e1 = expr THEN s2 = fstmt ELSE s3 = fstmt
-    { ErgoCompiler.sif (mk_position $startpos $endpos) e1 s2 s3 }
+    { ErgoCompiler.sif (mk_provenance $startpos $endpos) e1 s2 s3 }
 | ENFORCE e1 = expr ELSE s2 = fstmt SEMI s3 = fstmt
     { raise (LexError ("Cannot use enforce inside a function, you have to be in a Clause")) }
 | ENFORCE e1 = expr SEMI s3 = fstmt
@@ -304,7 +307,7 @@ fstmt:
 | EMIT e1 = expr SEMI s2 = fstmt
     { raise (LexError ("Cannot emit inside a function, you have to be in a Clause")) }
 | MATCH e0 = expr csd = cases_fstmt
-    { ErgoCompiler.smatch (mk_position $startpos $endpos) e0 (fst csd) (snd csd) }
+    { ErgoCompiler.smatch (mk_provenance $startpos $endpos) e0 (fst csd) (snd csd) }
 
 (* cases *)
 type_annotation:
@@ -343,97 +346,97 @@ expr:
     { e }
 (* Call *)
 | fn = IDENT LPAREN el = exprlist RPAREN
-    { ErgoCompiler.ecallfun (mk_position $startpos $endpos) (Util.char_list_of_string fn) el }
+    { ErgoCompiler.ecallfun (mk_provenance $startpos $endpos) (Util.char_list_of_string fn) el }
 (* Constants *)
 | NIL
-    { ErgoCompiler.econst (mk_position $startpos $endpos) ErgoCompiler.ErgoData.dunit }
+    { ErgoCompiler.econst (mk_provenance $startpos $endpos) ErgoCompiler.ErgoData.dunit }
 | TRUE
-    { ErgoCompiler.econst (mk_position $startpos $endpos) (ErgoCompiler.ErgoData.dbool true) }
+    { ErgoCompiler.econst (mk_provenance $startpos $endpos) (ErgoCompiler.ErgoData.dbool true) }
 | FALSE
-    { ErgoCompiler.econst (mk_position $startpos $endpos) (ErgoCompiler.ErgoData.dbool false) }
+    { ErgoCompiler.econst (mk_provenance $startpos $endpos) (ErgoCompiler.ErgoData.dbool false) }
 | i = INT
-    { ErgoCompiler.econst (mk_position $startpos $endpos) (ErgoCompiler.ErgoData.dnat (Util.coq_Z_of_int i)) }
+    { ErgoCompiler.econst (mk_provenance $startpos $endpos) (ErgoCompiler.ErgoData.dnat (Util.coq_Z_of_int i)) }
 | f = FLOAT
-    { ErgoCompiler.econst (mk_position $startpos $endpos) (ErgoCompiler.ErgoData.dfloat f) }
+    { ErgoCompiler.econst (mk_provenance $startpos $endpos) (ErgoCompiler.ErgoData.dfloat f) }
 | s = STRING
-    { ErgoCompiler.econst (mk_position $startpos $endpos) (ErgoCompiler.ErgoData.dstring (Util.char_list_of_string s)) }
+    { ErgoCompiler.econst (mk_provenance $startpos $endpos) (ErgoCompiler.ErgoData.dstring (Util.char_list_of_string s)) }
 | LBRACKET el = exprlist RBRACKET
-    { ErgoCompiler.earray (mk_position $startpos $endpos) el }
+    { ErgoCompiler.earray (mk_provenance $startpos $endpos) el }
 (* Expressions *)
 | v = IDENT
-    { ErgoCompiler.evar (mk_position $startpos $endpos) (Util.char_list_of_string v) }
+    { ErgoCompiler.evar (mk_provenance $startpos $endpos) (Util.char_list_of_string v) }
 | e = expr DOT a = safeident
-    { ErgoCompiler.edot (mk_position $startpos $endpos) a e }
+    { ErgoCompiler.edot (mk_provenance $startpos $endpos) a e }
 | e = expr QUESTIONDOT a = safeident
-    { ErgoCompiler.eoptionaldot (mk_position $startpos $endpos) a e }
+    { ErgoCompiler.eoptionaldot (mk_provenance $startpos $endpos) a e }
 | e1 = expr QUESTIONQUESTION e2 = expr
-    { ErgoCompiler.eoptionaldefault (mk_position $startpos $endpos) e1 e2 }
+    { ErgoCompiler.eoptionaldefault (mk_provenance $startpos $endpos) e1 e2 }
 | IF e1 = expr THEN e2 = expr ELSE e3 = expr
-    { ErgoCompiler.eif (mk_position $startpos $endpos) e1 e2 e3 }
+    { ErgoCompiler.eif (mk_provenance $startpos $endpos) e1 e2 e3 }
 | NEW qn = qname LCURLY r = reclist RCURLY
-    { ErgoCompiler.enew (mk_position $startpos $endpos) qn r }
+    { ErgoCompiler.enew (mk_provenance $startpos $endpos) qn r }
 | LCURLY r = reclist RCURLY
-    { ErgoCompiler.erecord (mk_position $startpos $endpos) r }
+    { ErgoCompiler.erecord (mk_provenance $startpos $endpos) r }
 | CONTRACT
-    { ErgoCompiler.ethis_contract (mk_position $startpos $endpos) }
+    { ErgoCompiler.ethis_contract (mk_provenance $startpos $endpos) }
 | CLAUSE
-    { ErgoCompiler.ethis_clause (mk_position $startpos $endpos) }
+    { ErgoCompiler.ethis_clause (mk_provenance $startpos $endpos) }
 | STATE
-    { ErgoCompiler.ethis_state (mk_position $startpos $endpos) }
+    { ErgoCompiler.ethis_state (mk_provenance $startpos $endpos) }
 | LET v = ident EQUAL e1 = expr SEMI e2 = expr
-    { ErgoCompiler.elet (mk_position $startpos $endpos) v None e1 e2 }
+    { ErgoCompiler.elet (mk_provenance $startpos $endpos) v None e1 e2 }
 | LET v = ident COLON t = paramtype EQUAL e1 = expr SEMI e2 = expr
-    { ErgoCompiler.elet (mk_position $startpos $endpos) v (Some t) e1 e2 }
+    { ErgoCompiler.elet (mk_provenance $startpos $endpos) v (Some t) e1 e2 }
 | MATCH e0 = expr csd = cases
-    { ErgoCompiler.ematch (mk_position $startpos $endpos) e0 (fst csd) (snd csd) }
+    { ErgoCompiler.ematch (mk_provenance $startpos $endpos) e0 (fst csd) (snd csd) }
 | FOREACH fl = foreachlist RETURN e2 = expr
-    { ErgoCompiler.eforeach (mk_position $startpos $endpos) fl None e2 }
+    { ErgoCompiler.eforeach (mk_provenance $startpos $endpos) fl None e2 }
 | FOREACH fl = foreachlist WHERE econd = expr RETURN e2 = expr
-    { ErgoCompiler.eforeach (mk_position $startpos $endpos) fl (Some econd) e2 }
+    { ErgoCompiler.eforeach (mk_provenance $startpos $endpos) fl (Some econd) e2 }
 (* Unary operators *)
 | MINUS e = expr %prec uminus
-    { ErgoCompiler.eunaryop (mk_position $startpos $endpos) ErgoCompiler.ErgoOps.Unary.Double.opuminus e }
+    { ErgoCompiler.eunaryop (mk_provenance $startpos $endpos) ErgoCompiler.ErgoOps.Unary.Double.opuminus e }
 | MINUSI e = expr %prec uminus
-    { ErgoCompiler.opuminusi (mk_position $startpos $endpos) e }
+    { ErgoCompiler.opuminusi (mk_provenance $startpos $endpos) e }
 | NOT e = expr
-    { ErgoCompiler.eunaryop (mk_position $startpos $endpos) ErgoCompiler.ErgoOps.Unary.opneg e }
+    { ErgoCompiler.eunaryop (mk_provenance $startpos $endpos) ErgoCompiler.ErgoOps.Unary.opneg e }
 (* Binary operators *)
 | e1 = expr EQUAL e2 = expr
-    { ErgoCompiler.ebinaryop (mk_position $startpos $endpos) ErgoCompiler.ErgoOps.Binary.opequal e1 e2 }
+    { ErgoCompiler.ebinaryop (mk_provenance $startpos $endpos) ErgoCompiler.ErgoOps.Binary.opequal e1 e2 }
 | e1 = expr NEQUAL e2 = expr
-    { ErgoCompiler.eunaryop (mk_position $startpos $endpos) ErgoCompiler.ErgoOps.Unary.opneg (ErgoCompiler.ebinaryop (mk_position $startpos $endpos) ErgoCompiler.ErgoOps.Binary.opequal e1 e2) }
+    { ErgoCompiler.eunaryop (mk_provenance $startpos $endpos) ErgoCompiler.ErgoOps.Unary.opneg (ErgoCompiler.ebinaryop (mk_provenance $startpos $endpos) ErgoCompiler.ErgoOps.Binary.opequal e1 e2) }
 | e1 = expr LT e2 = expr
-    { ErgoCompiler.ebinaryop (mk_position $startpos $endpos) ErgoCompiler.ErgoOps.Binary.oplt e1 e2 }
+    { ErgoCompiler.ebinaryop (mk_provenance $startpos $endpos) ErgoCompiler.ErgoOps.Binary.oplt e1 e2 }
 | e1 = expr LTEQ e2 = expr
-    { ErgoCompiler.ebinaryop (mk_position $startpos $endpos) ErgoCompiler.ErgoOps.Binary.ople e1 e2 }
+    { ErgoCompiler.ebinaryop (mk_provenance $startpos $endpos) ErgoCompiler.ErgoOps.Binary.ople e1 e2 }
 | e1 = expr GT e2 = expr
-    { ErgoCompiler.eunaryop (mk_position $startpos $endpos) ErgoCompiler.ErgoOps.Unary.opneg (ErgoCompiler.ebinaryop (mk_position $startpos $endpos) ErgoCompiler.ErgoOps.Binary.ople e1 e2) }
+    { ErgoCompiler.eunaryop (mk_provenance $startpos $endpos) ErgoCompiler.ErgoOps.Unary.opneg (ErgoCompiler.ebinaryop (mk_provenance $startpos $endpos) ErgoCompiler.ErgoOps.Binary.ople e1 e2) }
 | e1 = expr GTEQ e2 = expr
-    { ErgoCompiler.eunaryop (mk_position $startpos $endpos) ErgoCompiler.ErgoOps.Unary.opneg (ErgoCompiler.ebinaryop (mk_position $startpos $endpos) ErgoCompiler.ErgoOps.Binary.oplt e1 e2) }
+    { ErgoCompiler.eunaryop (mk_provenance $startpos $endpos) ErgoCompiler.ErgoOps.Unary.opneg (ErgoCompiler.ebinaryop (mk_provenance $startpos $endpos) ErgoCompiler.ErgoOps.Binary.oplt e1 e2) }
 | e1 = expr MINUS e2 = expr
-    { ErgoCompiler.ebinaryop (mk_position $startpos $endpos) ErgoCompiler.ErgoOps.Binary.Double.opminus e1 e2 }
+    { ErgoCompiler.ebinaryop (mk_provenance $startpos $endpos) ErgoCompiler.ErgoOps.Binary.Double.opminus e1 e2 }
 | e1 = expr PLUS e2 = expr
-    { ErgoCompiler.ebinaryop (mk_position $startpos $endpos) ErgoCompiler.ErgoOps.Binary.Double.opplus e1 e2 }
+    { ErgoCompiler.ebinaryop (mk_provenance $startpos $endpos) ErgoCompiler.ErgoOps.Binary.Double.opplus e1 e2 }
 | e1 = expr STAR e2 = expr
-    { ErgoCompiler.ebinaryop (mk_position $startpos $endpos) ErgoCompiler.ErgoOps.Binary.Double.opmult e1 e2 }
+    { ErgoCompiler.ebinaryop (mk_provenance $startpos $endpos) ErgoCompiler.ErgoOps.Binary.Double.opmult e1 e2 }
 | e1 = expr SLASH e2 = expr
-    { ErgoCompiler.ebinaryop (mk_position $startpos $endpos) ErgoCompiler.ErgoOps.Binary.Double.opdiv e1 e2 }
+    { ErgoCompiler.ebinaryop (mk_provenance $startpos $endpos) ErgoCompiler.ErgoOps.Binary.Double.opdiv e1 e2 }
 | e1 = expr CARROT e2 = expr
-    { ErgoCompiler.ebinaryop (mk_position $startpos $endpos) ErgoCompiler.ErgoOps.Binary.Double.oppow e1 e2 }
+    { ErgoCompiler.ebinaryop (mk_provenance $startpos $endpos) ErgoCompiler.ErgoOps.Binary.Double.oppow e1 e2 }
 | e1 = expr MINUSI e2 = expr
-    { ErgoCompiler.ebinaryop (mk_position $startpos $endpos) ErgoCompiler.ErgoOps.Binary.Integer.opminusi e1 e2 }
+    { ErgoCompiler.ebinaryop (mk_provenance $startpos $endpos) ErgoCompiler.ErgoOps.Binary.Integer.opminusi e1 e2 }
 | e1 = expr PLUSI e2 = expr
-    { ErgoCompiler.ebinaryop (mk_position $startpos $endpos) ErgoCompiler.ErgoOps.Binary.Integer.opplusi e1 e2 }
+    { ErgoCompiler.ebinaryop (mk_provenance $startpos $endpos) ErgoCompiler.ErgoOps.Binary.Integer.opplusi e1 e2 }
 | e1 = expr STARI e2 = expr
-    { ErgoCompiler.ebinaryop (mk_position $startpos $endpos) ErgoCompiler.ErgoOps.Binary.Integer.opmulti e1 e2 }
+    { ErgoCompiler.ebinaryop (mk_provenance $startpos $endpos) ErgoCompiler.ErgoOps.Binary.Integer.opmulti e1 e2 }
 | e1 = expr SLASHI e2 = expr
-    { ErgoCompiler.ebinaryop (mk_position $startpos $endpos) ErgoCompiler.ErgoOps.Binary.Integer.opdivi e1 e2 }
+    { ErgoCompiler.ebinaryop (mk_provenance $startpos $endpos) ErgoCompiler.ErgoOps.Binary.Integer.opdivi e1 e2 }
 | e1 = expr AND e2 = expr
-    { ErgoCompiler.ebinaryop (mk_position $startpos $endpos) ErgoCompiler.ErgoOps.Binary.opand e1 e2 }
+    { ErgoCompiler.ebinaryop (mk_provenance $startpos $endpos) ErgoCompiler.ErgoOps.Binary.opand e1 e2 }
 | e1 = expr OR e2 = expr
-    { ErgoCompiler.ebinaryop (mk_position $startpos $endpos) ErgoCompiler.ErgoOps.Binary.opor e1 e2 }
+    { ErgoCompiler.ebinaryop (mk_provenance $startpos $endpos) ErgoCompiler.ErgoOps.Binary.opor e1 e2 }
 | e1 = expr PLUSPLUS e2 = expr
-    { ErgoCompiler.ebinaryop (mk_position $startpos $endpos) ErgoCompiler.ErgoOps.Binary.opstringconcat e1 e2 }
+    { ErgoCompiler.ebinaryop (mk_provenance $startpos $endpos) ErgoCompiler.ErgoOps.Binary.opstringconcat e1 e2 }
 
 (* foreach list *)
 foreachlist:
