mechanization/Common/Utils/EProvenance.v
@@ -1,0 +1,76 @@
+(*
+ * Licensed under the Apache License, Version 2.0 (the "License");
+ * you may not use this file except in compliance with the License.
+ * You may obtain a copy of the License at
+ *
+ * http://www.apache.org/licenses/LICENSE-2.0
+ *
+ * Unless required by applicable law or agreed to in writing, software
+ * distributed under the License is distributed on an "AS IS" BASIS,
+ * WITHOUT WARRANTIES OR CONDITIONS OF ANY KIND, either express or implied.
+ * See the License for the specific language governing permissions and
+ * limitations under the License.
+ *)
+
+(* Provenance and location *)
+
+Require Import String.
+Require Import ZArith.
+
+Section EProvenance.
+  Record location_point :=
+    mkLocationPoint {
+        offset: Z;
+        line : Z;
+        column : Z;
+      }.
+  Record location :=
+    mkLocation {
+        loc_file: option string;
+        loc_start: location_point;
+        loc_end: location_point;
+      }.
+  Definition dummy_location : location :=
+    let dummy_location_point := mkLocationPoint (-1) (-1) (-1) in
+    mkLocation None dummy_location_point dummy_location_point.
+
+  (* Provenance *)
+  Inductive provenance :=
+  | ProvFunc : location -> string -> provenance   (**r Compiled from function *)
+  | ProvClause : location -> string -> provenance (**r Compiled from clause *)
+  | ProvThisContract : location -> provenance     (**r Compiled from [contract] *)
+  | ProvThisClause : location -> provenance       (**r Compiled from [clause] *)
+  | ProvThisState : location -> provenance        (**r Compiled from [state] *)
+  | ProvLoc : location -> provenance              (**r Compiled from others *)
+  .
+
+  Definition dummy_provenance : provenance :=
+    ProvLoc dummy_location.
+
+  Definition loc_of_provenance prov : location :=
+    match prov with
+    | ProvFunc loc _ => loc
+    | ProvClause loc _ => loc
+    | ProvThisContract loc => loc
+    | ProvThisClause loc => loc
+    | ProvThisState loc => loc
+    | ProvLoc loc => loc
+    end.
+
+  Definition is_contract prov : bool :=
+    match prov with
+    | ProvThisContract loc => true
+    | _ => false
+    end.
+  Definition is_clause prov : bool :=
+    match prov with
+    | ProvThisClause loc => true
+    | _ => false
+    end.
+  Definition is_state prov : bool :=
+    match prov with
+    | ProvThisState loc => true
+    | _ => false
+    end.
+    
+End EProvenance.
