mechanization/Ergo/Lang/ErgoSugar.v
@@ -25,78 +25,30 @@ Require Import ErgoSpec.Ergo.Lang.Ergo.
 Require Import ErgoSpec.Backend.ErgoBackend.
 
 Section ErgoSugar.
-  Section ParserSugar.
-    Context {A:Set}. (* Type for annotations *)
+  Context {A:Set}. (* Type for annotations *)
   
-    (** [expr.field] is a macro for unbranding followed by field access in a record *)
-    Definition EDot (a:A) (s:string) (e:rergo_expr) : rergo_expr :=
-      EUnaryOp a
-               (ErgoOps.Unary.opdot s)
-               (EUnaryOp a ErgoOps.Unary.opunbrand e).
+  (** [expr.field] is a macro for unbranding followed by field access in a record *)
+  Definition EDot (a:A) (s:string) (e:rergo_expr) : rergo_expr :=
+    EUnaryOp a
+             (ErgoOps.Unary.opdot s)
+             (EUnaryOp a ErgoOps.Unary.opunbrand e).
 
-    Definition SReturnEmpty (a:A) : rergo_stmt :=
-      SReturn a (EConst a dunit).
-  
-    Definition SFunReturnEmpty (a:A) : rergo_stmt :=
-      SFunReturn a (EConst a dunit).
+  Definition SReturnEmpty (a:A) : rergo_stmt :=
+    SReturn a (EConst a dunit).
 
-    Definition EOptionalDot (a:A) (pname:string) (e:rergo_expr) :=
-      EMatch a
-             e
-             ((CaseLetOption "$option" None,
-               EUnaryOp a (OpDot pname) (EVar a "$option")) :: nil)
-             (EConst a dnone).
-    Definition EOptionalDefault (a:A) (e1 e2:rergo_expr) :=
-      EMatch a e1
-             ((CaseLetOption "$option" None, EVar a "$option") :: nil)
-             e2.
+  Definition SFunReturnEmpty (a:A) : rergo_stmt :=
+    SFunReturn a (EConst a dunit).
 
-    (*
-    Definition SThrowSugar (loc:location) (ns:namespace_prefix) (ln:local_name) (el:list (string*laergo_expr)) : laergo_stmt :=
-      SThrow loc (ENew loc (ns,ln) el).
-*)
+  Definition EOptionalDot (a:A) (pname:string) (e:rergo_expr) :=
+    EMatch a
+           e
+           ((CaseLetOption "$option" None,
+             EUnaryOp a (OpDot pname) (EVar a "$option")) :: nil)
+           (EConst a dnone).
 
-    (*
-    Definition SThrowErgoCompilerError (a:A) (msg:string) : rergo_stmt :=
-      SThrowSugar a
-                  (Some "org.ergo"%string)
-                  "Error"%string
-                  (("error"%string, EConst a (ErgoData.dstring msg))::nil).
-*)
-
-  End ParserSugar.
-
-  Section StmtSugar.
-    (** [return expr] is a no-op at the moment *)
-    Definition mk_result (loc:location) e1 e2 e3 : laergo_expr :=
-      ERecord loc
-              ((this_response, e1)
-                 :: (this_state, e2)
-                 :: (this_emit, e3)
-                 :: nil).
-
-    Definition set_state (loc:location) e1 e2 : laergo_expr :=
-      ELet loc local_state None e1 e2.
-
-    Definition this_clause (loc:location) clause_name : laergo_expr :=
-      EUnaryOp loc
-               (OpDot clause_name)
-               (EUnaryOp loc OpUnbrand (EThisContract loc)).
-
-    Definition push_emit (loc:location) e1 e2 : laergo_expr :=
-      ELet loc local_emit None
-           (EBinaryOp loc
-                      OpBagUnion
-                      (EUnaryOp loc OpBag e1)
-                      (EVar loc local_emit))
+  Definition EOptionalDefault (a:A) (e1 e2:rergo_expr) :=
+    EMatch a e1
+           ((CaseLetOption "$option" None, EVar a "$option") :: nil)
            e2.
-
-    Definition ESuccess (loc:location) (e:laergo_expr) : laergo_expr :=
-      EUnaryOp loc OpLeft e.
-      
-    Definition EError (loc:location) (e:laergo_expr) : laergo_expr :=
-      EUnaryOp loc OpRight e.
-
-  End StmtSugar.
 
 End ErgoSugar.
