mechanization/ErgoCalculus/Lang/ErgoCalculusSugar.v
@@ -1,0 +1,68 @@
+(*
+ * Licensed under the Apache License, Version 2.0 (the "License");
+ * you may not use this file except in compliance with the License.
+ * You may obtain a copy of the License at
+ *
+ * http://www.apache.org/licenses/LICENSE-2.0
+ *
+ * Unless required by applicable law or agreed to in writing, software
+ * distributed under the License is distributed on an "AS IS" BASIS,
+ * WITHOUT WARRANTIES OR CONDITIONS OF ANY KIND, either express or implied.
+ * See the License for the specific language governing permissions and
+ * limitations under the License.
+ *)
+
+(** Ergo is a language for expressing contract logic. *)
+
+(** * Syntactic sugar *)
+
+Require Import String.
+Require Import List.
+Require Import ErgoSpec.Common.Utils.EProvenance.
+Require Import ErgoSpec.Common.Utils.ENames.
+Require Import ErgoSpec.Common.Utils.EResult.
+Require Import ErgoSpec.Common.Pattern.EPattern.
+Require Import ErgoSpec.Ergo.Lang.Ergo.
+Require Import ErgoSpec.ErgoCalculus.Lang.ErgoCalculus.
+Require Import ErgoSpec.Backend.ErgoBackend.
+
+Section ErgoCalculusSugar.
+  Definition mkResult (prov:provenance) e1 e2 e3 : ergoc_expr :=
+    ERecord prov
+            ((this_response, e1)
+               :: (this_state, e2)
+               :: (this_emit, e3)
+               :: nil).
+
+  Definition setState (prov:provenance) e1 e2 : ergoc_expr :=
+    ELet prov local_state None e1 e2.
+
+  Definition thisContract (prov:provenance) : ergoc_expr :=
+    let prov := ProvThisContract (loc_of_provenance prov) in
+    EVar prov this_contract.
+
+  Definition thisClause (prov:provenance) clause_name : ergoc_expr :=
+    let prov := ProvThisClause (loc_of_provenance prov) in
+    EUnaryOp prov
+             (OpDot clause_name)
+             (EUnaryOp prov OpUnbrand (EVar prov this_contract)).
+
+  Definition thisState (prov:provenance) : ergoc_expr :=
+    let prov := ProvThisState (loc_of_provenance prov) in
+    EVar prov local_state.
+
+  Definition pushEmit (prov:provenance) e1 e2 : ergoc_expr :=
+    ELet prov local_emit None
+         (EBinaryOp prov
+                    OpBagUnion
+                    (EUnaryOp prov OpBag e1)
+                    (EVar prov local_emit))
+         e2.
+
+  Definition ESuccess (prov:provenance) (e:ergoc_expr) : ergoc_expr :=
+    EUnaryOp prov OpLeft e.
+
+  Definition EError (prov:provenance) (e:ergoc_expr) : ergoc_expr :=
+    EUnaryOp prov OpRight e.
+
+End ErgoCalculusSugar.
