mechanization/ErgoNNRC/Lang/ErgoNNRCCall.v
@@ -16,10 +16,9 @@ Require Import String.
 Require Import List.
 
 Require Import Qcert.Utils.ListAdd. (* For zip *)
-Require Import Qcert.Utils.Lift.
-Require Qcert.Utils.Closure.
 
 Require Import ErgoSpec.Backend.ErgoBackend.
+Require Import ErgoSpec.Common.Utils.EProvenance.
 Require Import ErgoSpec.Common.Utils.ENames.
 Require Import ErgoSpec.Common.Utils.EResult.
 Require Import ErgoSpec.Common.Types.ErgoType.
@@ -43,20 +42,20 @@ Section Lambda.
 End Lambda.
 
 Section Patch.
-  Definition nnrc_lambda_type_of_lambda_type (loc:location) (t:option unit) : nnrc_type :=
-    ErgoTypeAny loc.
+  Definition nnrc_lambda_type_of_lambda_type (prov:provenance) (t:option unit) : nnrc_type :=
+    ErgoTypeAny prov.
 
   Definition nnrc_lambda_params_of_lambda_params
-             (loc:location)
+             (prov:provenance)
              (params:list (string * option unit)) : list (string * nnrc_type) :=
-    List.map (fun xy => (fst xy, nnrc_lambda_type_of_lambda_type loc (snd xy))) params.
+    List.map (fun xy => (fst xy, nnrc_lambda_type_of_lambda_type prov (snd xy))) params.
     
   Definition nnrc_expr_lambda_of_backend_closure
              (cl:ErgoEnhancedBackend.ergo_backend_closure) : nnrc_expr_lambda :=
-    let loc := dummy_location in (* XXX TO DECIDE *)
+    let prov := dummy_provenance in (* XXX TO DECIDE *)
     mkLambdaN
-      (nnrc_lambda_params_of_lambda_params loc cl.(Closure.closure_params))
-      (nnrc_lambda_type_of_lambda_type loc cl.(Closure.closure_output))
+      (nnrc_lambda_params_of_lambda_params prov cl.(Closure.closure_params))
+      (nnrc_lambda_type_of_lambda_type prov cl.(Closure.closure_output))
       cl.(Closure.closure_body).
 
   Definition lookup_table_of_backend_lookup_table
@@ -87,17 +86,17 @@ Section ErgoNNRCCall.
 
   (** Looks up a function with its parameters. If the function exists and the number of parameters
       is correct, it returns a closed expression computing the call. *)
-  Definition lookup_lambda (loc:location) (t:lookup_table) (fname:string) : eresult nnrc_expr_lambda :=
+  Definition lookup_lambda (prov:provenance) (t:lookup_table) (fname:string) : eresult nnrc_expr_lambda :=
     match t fname with
-    | None => function_not_found_error loc fname
+    | None => function_not_found_error prov fname
     | Some cl => esuccess cl
     end.
 
-  Definition lookup_call (loc:location) (t:lookup_table) (fname:string) (el:list nnrc_expr) : eresult nnrc_expr :=
-    let rlambda := lookup_lambda loc t fname in
+  Definition lookup_call (prov:provenance) (t:lookup_table) (fname:string) (el:list nnrc_expr) : eresult nnrc_expr :=
+    let rlambda := lookup_lambda prov t fname in
     eolift (fun cl =>
              match zip_params (List.map fst cl.(lambdan_params)) el with
-             | None => call_params_error loc fname
+             | None => call_params_error prov fname
              | Some params => 
                esuccess (create_call params cl.(lambdan_body))
              end) rlambda.
